ironfleet/ravana/RefinementProof/Node_SwitchRecvCommand.dfy
@@ -1,0 +1,283 @@
+include "../Types.i.dfy"
+include "../Refinement.i.dfy"
+include "../Service.i.dfy"
+include "../DistributedSystem.i.dfy"
+include "../RefinementLemmas.i.dfy"
+
+module Refinement_Proof_InitNewMaster {
+  import opened Types_i
+  import opened Refinement_i
+  import opened Service_i
+  import opened DistributedSystem_i
+  import opened RefinementLemmas_i
+
+  predicate conditions(rs: RState, rs': RState)
+  {
+    rstate_valid(rs)
+
+    && LEnvironment_Next(rs.environment, rs'.environment)
+    && rs.environment.nextStep.LEnvStepHostIos?
+    && rs.endpoint_logger == rs'.endpoint_logger
+    && rs.initControllerState == rs'.initControllerState
+    && rs.environment.nextStep.actor in rs.server_switches
+    && rs.environment.nextStep.actor in rs'.server_switches
+    && Node_SwitchRecvCommand(
+                rs.server_switches[rs.environment.nextStep.actor],
+                rs'.server_switches[rs.environment.nextStep.actor],
+                rs.environment.nextStep.ios)
+    && rs.server_controllers == rs'.server_controllers
+    && rs.server_logger == rs'.server_logger
+    && rs'.server_switches == rs.server_switches[
+        rs.environment.nextStep.actor := rs'.server_switches[rs.environment.nextStep.actor]]
+  }
+
+  lemma lemma_refines_SwitchEventSend(rs: RState, rs': RState)
+  requires conditions(rs, rs')
+
+  ensures rstate_valid(rs')
+  ensures Service_NextApplyCommand(refinement(rs), refinement(rs'))
+  {
+    lemma_packets_are_valid(rs, rs');
+    lemma_log_is_valid(rs, rs');
+    lemma_accepted_commands_are_valid(rs, rs');
+    lemma_switches_valid(rs, rs');
+
+    lemma_outstanding_events_eq(rs, rs');
+
+    var sc := SingleCommand(rs.environment.nextStep.actor,
+                            rs.environment.nextStep.ios[0].r.msg.command);
+
+    lemma_multiset(rs, rs', sc);
+  }
+
+  lemma {:axiom} lemma_packets_are_valid(rs: RState, rs': RState)
+  requires conditions(rs, rs')
+  ensures packets_are_valid(rs')
+  /*
+  {
+    packet_validation_preservation(rs, rs');
+    lemma_packets_are_valid_no_sending(rs, rs');
+  }
+  */
+
+  lemma {:axiom} packet_validation_preservation(rs: RState, rs': RState)
+  requires conditions(rs, rs')
+  ensures packet_validation_preserved(rs, rs')
+  /*
+  {
+    forall p : LPacket<EndPoint, RavanaMessage>
+    ensures 
+        is_valid_message(rs, p.src, p.dst, p.msg) ==>
+        is_valid_message(rs', p.src, p.dst, p.msg)
+    {
+      if (is_valid_message(rs, p.src, p.dst, p.msg)) {
+        match p.msg
+          case EventMessage(event: Event, event_id: int) => {
+            assert is_valid_EventMessage(rs', p.src, p.dst, p.msg);
+          }
+          case EventAck(event_ack_id: int) => {
+            assert is_valid_EventAck(rs', p.src, p.dst, p.msg);
+          }
+          case CommandMessage(command: Command, command_id: int) => {
+            assert is_valid_CommandMessage(rs', p.src, p.dst, p.msg);
+          }
+          case CommandAck(command_ack_id: int) => {
+            assert is_valid_CommandAck(rs', p.src, p.dst, p.msg);
+          }
+          case InitNewMaster(leader_id: int) => {
+            assert is_valid_InitNewMaster(rs', p.src, p.dst, p.msg);
+          }
+          case NewMaster(master_id: int) => {
+            assert is_valid_NewMaster(rs', p.src, p.dst, p.msg);
+          }
+          case NewMasterAck => {
+            assert is_valid_NewMasterAck(rs', p.src, p.dst, p.msg);
+          }
+          case LogMessage(log_entry: LogEntry) => {
+            assert is_valid_LogMessage(rs', p.src, p.dst, p.msg);
+          }
+          case LogBroadcastMessage(full_log: seq<LogEntry>) => {
+            assert is_valid_LogBroadcastMessage(rs', p.src, p.dst, p.msg);
+          }
+      }
+    }
+    reveal_packet_validation_preserved();
+  }
+  */
+
+  lemma {:axiom} lemma_log_is_valid(rs: RState, rs': RState)
+  requires conditions(rs, rs')
+  ensures log_is_valid(rs'.server_switches, rs'.server_logger.log)
+  /*
+  {
+    reveal_log_is_valid();
+  }
+  */
+
+  lemma {:axiom} lemma_accepted_commands_are_valid(rs: RState, rs': RState)
+  requires conditions(rs, rs')
+  ensures accepted_commands_are_valid(rs'.initControllerState,
+        rs'.server_switches, rs'.server_logger.log)
+  /*
+  {
+    reveal_accepted_commands_are_valid();
+
+    var all_commands := controller_state_looking_forward(
+                rs'.server_logger.log, rs'.initControllerState).commands;
+
+    var s := rs.server_switches[rs.environment.nextStep.actor];
+
+    forall ep | ep in rs'.server_switches
+      ensures forall command_id :: command_id in rs'.server_switches[ep].received_command_ids ==>
+        0 <= command_id < |all_commands| &&
+        all_commands[command_id].switch == ep
+    {
+      forall command_id | command_id in rs'.server_switches[ep].received_command_ids
+      ensures 0 <= command_id < |all_commands|
+      ensures all_commands[command_id].switch == ep
+      {
+        if (ep != rs.environment.nextStep.actor) {
+          assert 0 <= command_id < |all_commands|;
+          assert all_commands[command_id].switch == ep;
+        } else {
+          assert command_id in (s.received_command_ids +
+              [rs.environment.nextStep.ios[0].r.msg.command_id]);
+          if (command_id in s.received_command_ids) {
+            assert 0 <= command_id < |all_commands|;
+            assert all_commands[command_id].switch == ep;
+          } else {
+            assert command_id == rs.environment.nextStep.ios[0].r.msg.command_id;
+            lemma_valid_command_msg(rs, rs');
+            assert 0 <= command_id < |all_commands|;
+            assert all_commands[command_id].switch == ep;
+          }
+        }
+      }
+    }
+  }
+  */
+
+  lemma {:axiom} lemma_valid_command_msg(rs: RState, rs': RState)
+  requires conditions(rs, rs')
+  ensures is_valid_CommandMessage(rs,
+      rs.environment.nextStep.ios[0].r.src,
+      rs.environment.nextStep.ios[0].r.dst,
+      rs.environment.nextStep.ios[0].r.msg)
+  /*
+  {
+    reveal_packets_are_valid();
+  }
+  */
+
+  lemma {:axiom} lemma_switches_valid(rs: RState, rs': RState)
+  requires conditions(rs, rs')
+  ensures switches_valid(rs'.server_switches)
+  /*
+  {
+    reveal_switches_valid();
+  }
+  */
+
+  lemma {:axiom} lemma_multiset(rs: RState, rs': RState, sc: SingleCommand)
+  requires conditions(rs, rs')
+  requires rstate_valid(rs')
+  requires sc == SingleCommand(rs.environment.nextStep.actor,
+                               rs.environment.nextStep.ios[0].r.msg.command)
+  ensures multiset_adds_one(
+      refinement(rs').outstandingCommands,
+      refinement(rs).outstandingCommands)
+  ensures sc == added_obj(
+      refinement(rs').outstandingCommands,
+      refinement(rs).outstandingCommands)
+  /*
+  {
+    lemma_multiset_inc(rs, rs', sc);
+    reveal_added_obj();
+  }
+  */
+
+  lemma {:axiom} lemma_multiset_inc(rs: RState, rs': RState, sc: SingleCommand)
+  requires conditions(rs, rs')
+  requires rstate_valid(rs')
+  requires sc == SingleCommand(rs.environment.nextStep.actor,
+                               rs.environment.nextStep.ios[0].r.msg.command)
+  ensures refinement_outstandingCommands(rs.server_logger.log, rs.initControllerState, rs.server_switches)
+       == refinement_outstandingCommands(rs'.server_logger.log, rs'.initControllerState, rs'.server_switches) + multiset{sc}
+       /* 
+  {
+    lemma_incoming_command_matches_log(rs, rs', sc,
+              rs.environment.nextStep.ios[0].r.msg.command_id);
+    lemma_filter_out_accepted_commands_inc(rs, rs', sc,
+              rs.environment.nextStep.ios[0].r.msg.command_id,
+              controller_state_looking_forward(
+                rs'.server_logger.log, rs'.initControllerState).commands);
+    assert refinement_outstandingCommands(rs.server_logger.log, rs.initControllerState, rs.server_switches)
+        == filter_out_accepted_commands(controller_state_looking_forward(
+              rs.server_logger.log, rs.initControllerState).commands, rs.server_switches)
+        == filter_out_accepted_commands(controller_state_looking_forward(
+              rs'.server_logger.log, rs'.initControllerState).commands, rs'.server_switches)
+            + multiset{sc}
+        == refinement_outstandingCommands(rs'.server_logger.log, rs'.initControllerState, rs'.server_switches)
+            + multiset{sc};
+  }
+  */
+
+  lemma {:axiom} lemma_filter_out_accepted_commands_inc(
+      rs: RState, rs': RState, sc: SingleCommand, idx: int, comms: seq<SingleCommand>)
+  requires conditions(rs, rs')
+  requires rstate_valid(rs')
+  requires 0 <= idx < |comms|
+  requires comms[idx] == sc
+  requires sc.switch in rs.server_switches
+  requires !(idx in rs.server_switches[sc.switch].received_command_ids)
+  requires rs'.server_switches[sc.switch].received_command_ids ==
+             rs.server_switches[sc.switch].received_command_ids + [idx]
+  ensures  filter_out_accepted_commands(comms, rs.server_switches)
+        == filter_out_accepted_commands(comms, rs'.server_switches)
+            + multiset{sc}
+  /*
+  {
+    assert |comms| != 0;
+    if (idx == |comms| - 1) {
+      lemma_filter_out_accepted_commands_inc2(rs, rs', sc, idx, comms[0 .. |comms| - 1]);
+    } else {
+      lemma_filter_out_accepted_commands_inc(rs, rs', sc, idx, comms[0 .. |comms| - 1]);
+    }
+  }
+  */
+
+  lemma {:axiom} lemma_filter_out_accepted_commands_inc2(
+      rs: RState, rs': RState, sc: SingleCommand, idx: int, comms: seq<SingleCommand>)
+  requires conditions(rs, rs')
+  requires rstate_valid(rs')
+  requires |comms| <= idx
+  requires sc.switch in rs.server_switches
+  requires !(idx in rs.server_switches[sc.switch].received_command_ids)
+  requires rs'.server_switches[sc.switch].received_command_ids ==
+             rs.server_switches[sc.switch].received_command_ids + [idx]
+  ensures  filter_out_accepted_commands(comms, rs.server_switches)
+        == filter_out_accepted_commands(comms, rs'.server_switches)
+  /*
+  {
+    if (|comms| == 0) {
+    } else {
+      lemma_filter_out_accepted_commands_inc2(rs, rs', sc, idx, comms[0 .. |comms| - 1]);
+    }
+  }
+  */
+
+  lemma lemma_incoming_command_matches_log(rs: RState, rs': RState, sc: SingleCommand,
+      command_id: int)
+  requires conditions(rs, rs')
+  requires rstate_valid(rs')
+  requires command_id == rs.environment.nextStep.ios[0].r.msg.command_id
+  requires sc == SingleCommand(rs.environment.nextStep.actor,
+                               rs.environment.nextStep.ios[0].r.msg.command)
+  ensures 0 <= command_id < |controller_state_looking_forward(
+                rs.server_logger.log, rs.initControllerState).commands|
+  ensures controller_state_looking_forward(
+                rs.server_logger.log, rs.initControllerState).commands[command_id] == sc
+  {
+    lemma_valid_command_msg(rs, rs');
+  }
+}
